Summing the N Series
====================

You are given a series, whose n<sup>th</sup> term is defined as

T<sub>n</sub> = n<sup>2</sup> - (n - 1)<sup>2</sup>

You have to find the Sum of the series S<sub>n</sub> = T<sub>1</sub> + T<sub>2</sub> + T<sub>3</sub> + ... + T<sub>n</sub>

Find S<sub>n</sub> % (10<sup>9</sup> + 7)

### Input:

First line contains `T`, denoting the number of testcases.

Each test case contains 1 line:

`n`

### Output:

Print the required sum % (10<sup>9</sup> + 7).

### Constraints:

* 1 <= T <= 10
* 1 <= n <= 10<sup>16</sup>

### Sample Input:

    2
    2
    1

### Sample Output:

    4
    1

### Explanation:

Case #00: We have 4 = 1 + 3

Case #01: We have 1 = 1
